Tuned

Snippets.thy
@@ -4,11 +4,11 @@ begin
 
   section \<open>Find Element in Array (Arrays)\<close>
 
-  definition "find_elem (x::int) xs \<equiv> do {
+  definition "find_elem (x::int) xs \<equiv> doN {
     WHILEIT (\<lambda>i. i\<le>length xs \<and> x\<notin>set (take i xs)) (\<lambda>i. i<length xs \<and> xs!i\<noteq>x) (\<lambda>i. RETURN (i+1)) 0
   }"
   
-  lemma "find_elem x xs \<le> SPEC (\<lambda>i. i\<le>length xs \<and> (i<length xs \<longrightarrow> xs!i = x))"
+  lemma find_elem_correct: "find_elem x xs \<le> SPEC (\<lambda>i. i\<le>length xs \<and> (i<length xs \<longrightarrow> xs!i = x))"
     unfolding find_elem_def
     apply refine_vcg
     apply (rule wf_measure[of "\<lambda>i. length xs - i"])
@@ -22,6 +22,13 @@ begin
   
   export_code find_elem_impl in Haskell module_name test
 
+  
+  subsection \<open>Combined Correctness Theorem\<close>  
+  lemma find_elem_r1: "(find_elem, \<lambda> x xs. SPEC (\<lambda>i. i\<le>length xs \<and> (i<length xs \<longrightarrow> xs!i = x))) \<in> Id \<rightarrow> Id \<rightarrow> \<langle>Id\<rangle>nres_rel"
+    using find_elem_correct by (auto intro: nres_relI)
+  
+  thm find_elem_impl.refine[FCOMP find_elem_r1]
+  
 
   section \<open>Check Prefix (Arrays, Exceptions: Check)\<close>
     
@@ -36,7 +43,7 @@ begin
   }"
   
   (* ESPEC Exc Normal ! *)
-  lemma "check_prefix xs ys \<le> ESPEC (\<lambda>_. xs \<noteq> take (length xs) ys) (\<lambda>_. xs = take (length xs) ys)"
+  lemma check_prefix_correct: "check_prefix xs ys \<le> ESPEC (\<lambda>_. xs \<noteq> take (length xs) ys) (\<lambda>_. xs = take (length xs) ys)"
     unfolding check_prefix_def
     apply (refine_vcg EWHILEIT_rule[where R="measure (\<lambda>i. length xs - i)"])
     apply auto []
@@ -69,19 +76,54 @@ begin
     by sepref
   
   export_code check_prefix_impl checking SML_imp
+
+  subsection \<open>Modularity\<close>
+    
+  lemmas [refine_vcg] = check_prefix_correct[THEN ESPEC_trans]
+  thm SPEC_trans (* for plain nres-monad without exceptions *)
+    
+  (* TODO: I remember to have automated the order_trans transformation, but cannot find it right now. *)
   
+
+  definition "is_prefix' xs ys \<equiv> CATCH (doE {check_prefix xs ys; ERETURN True }) (\<lambda>_. ERETURN False)"  
+  
+  lemma is_prefix'_correct: "is_prefix' xs ys \<le> ESPEC (\<lambda>_. False) (\<lambda>r. r \<longleftrightarrow> xs = take (length xs) ys)"
+    unfolding is_prefix'_def
+    apply refine_vcg
+    by auto
+  
+  lemmas [sepref_fr_rules] = check_prefix_impl.refine  
+  sepref_register check_prefix_bd :: "'a list \<Rightarrow> 'a list \<Rightarrow> (unit+unit) nres"
+    (* Optional interface type. Required if interfaces used that do not match Isabelle types, e.g. i_map, i_mtx, \<dots>*)
+
+  synth_definition is_prefix_bd' is [enres_unfolds]: "is_prefix' xs ys = \<hole>"
+    apply (rule CNV_eqD)
+    unfolding is_prefix'_def
+    apply opt_enres_unfold
+    apply (rule CNV_I)
+    done
+    
+  sepref_definition is_prefix_impl' is "uncurry is_prefix_bd'" 
+    :: "(array_assn int_assn)\<^sup>k *\<^sub>a (array_assn int_assn)\<^sup>k \<rightarrow>\<^sub>a (unit_assn +\<^sub>a bool_assn)"
+    unfolding is_prefix_bd'_def
+    by sepref
+  
+  export_code is_prefix_impl' checking SML_imp
+  
+  
+      
 
   section \<open>Is Prefix (Arrays, Exceptions: Catch)\<close>
   
   definition "is_prefix xs ys \<equiv> CATCH (doE {
-    CHECK (length xs \<le> length ys) ();
+    CHECK (length xs \<le> length ys) False;
     EWHILEIT (\<lambda>i. i\<le>length xs \<and> take i xs = take i ys) (\<lambda>i. i<length xs) (\<lambda>i. doE { 
       EASSERT (i<length xs \<and> i<length ys); 
-      CHECK (xs!i = ys!i) (); 
+      CHECK (xs!i = ys!i) False;
       ERETURN (i+1) 
     } ) 0;
-    ERETURN True
-  }) (\<lambda>_. ERETURN False)"
+    THROW True
+  }) (ERETURN)"
   
   (* ESPEC Exc Normal ! *)
   lemma "is_prefix xs ys \<le> ESPEC (\<lambda>_. False) (\<lambda>r. r \<longleftrightarrow> xs = take (length xs) ys)"
@@ -128,17 +170,50 @@ begin
   
   section \<open>Copy Array (Arrays, For i=l..u)\<close>  
   
-  definition "cp_array xs \<equiv> do {
+  definition "cp_array xs \<equiv> doN {
     let ys = op_array_replicate (length xs) 0;   (* Use proper constructors *)
     
-    ys \<leftarrow> nfoldli [0..<length xs] (\<lambda>_. True) (\<lambda>i ys. do {  (* Ensure linearity! ys\<leftarrow>\<dots> *)
+    ys \<leftarrow> nfoldli [0..<length xs] (\<lambda>_. True) (\<lambda>i ys. doN {  (* Ensure linearity! ys\<leftarrow>\<dots> *)
       ASSERT (i<length xs \<and> i<length ys); 
       RETURN (ys[i:=xs!i]) 
     }) ys;
     
     RETURN ys
   }"
+
   
+  lemma "cp_array xs \<le> SPEC (\<lambda>ys. ys=xs)"
+    unfolding cp_array_def
+    supply nfoldli_rule nfoldli_rule[where I="\<lambda>l1 l2 ys. length ys = length xs \<and> (\<forall>i\<in>set l1. ys!i = xs!i)", refine_vcg]
+    apply refine_vcg
+    apply auto
+    subgoal 
+      using upt_eq_lel_conv by blast
+    subgoal
+      using upt_eq_lel_conv by blast
+    subgoal 
+      by (simp add: nth_list_update)
+    subgoal 
+      by (simp add: nth_equalityI)
+    done  
+    
+
+  term arl_assn  
+    
+  subsection \<open>Proof with \<open>nfoldli_upt_rule\<close>\<close>  
+  lemma "cp_array xs \<le> SPEC (\<lambda>ys. ys=xs)"
+    unfolding cp_array_def
+    supply nfoldli_upt_rule nfoldli_upt_rule[where I="\<lambda>i ys. length ys = length xs \<and> (\<forall>j<i. ys!j = xs!j)", refine_vcg]
+    apply refine_vcg
+    apply auto
+    subgoal
+      using less_Suc_eq by auto 
+    subgoal
+      by (simp add: nth_equalityI)
+    done
+      
+  
+    
   sepref_definition cp_array_impl is cp_array :: "(array_assn nat_assn)\<^sup>k \<rightarrow>\<^sub>a array_assn nat_assn"
     unfolding cp_array_def
     by sepref
