VTcomp.thy
@@ -10,5 +10,86 @@ begin
 no_notation Ref.lookup ("!_" 61)
 no_notation Ref.update ("_ := _" 62)
 
+section \<open>Added Stuff\<close>
+
+lemma nfoldli_upt_rule:
+  assumes INTV: "lb\<le>ub"
+  assumes I0: "I lb \<sigma>0"
+  assumes IS: "\<And>i \<sigma>. \<lbrakk> lb\<le>i; i<ub; I i \<sigma>; c \<sigma> \<rbrakk> \<Longrightarrow> f i \<sigma> \<le> SPEC (I (i+1))"
+  assumes FNC: "\<And>i \<sigma>. \<lbrakk> lb\<le>i; i\<le>ub; I i \<sigma>; \<not>c \<sigma> \<rbrakk> \<Longrightarrow> P \<sigma>"
+  assumes FC: "\<And>\<sigma>. \<lbrakk> I ub \<sigma>; c \<sigma> \<rbrakk> \<Longrightarrow> P \<sigma>"
+  shows "nfoldli [lb..<ub] c f \<sigma>0 \<le> SPEC P"
+  apply (rule nfoldli_rule[where I="\<lambda>l _ \<sigma>. I (lb+length l) \<sigma>"])
+  apply simp_all
+  apply (simp add: I0)
+  subgoal using IS
+    by (metis Suc_eq_plus1 add_diff_cancel_left' eq_diff_iff le_add1 length_upt upt_eq_lel_conv)
+  subgoal for l1 l2 \<sigma> 
+    apply (rule FNC[where i="lb + length l1"])
+    apply (auto simp: INTV)
+    using INTV upt_eq_append_conv by auto
+  apply (rule FC) using INTV 
+  by auto  
+
+term Refine_Basic.bind
+  
+abbreviation (do_notation) bind_doN where "bind_doN \<equiv> Refine_Basic.bind"
+
+notation (output) bind_doN (infixr "\<bind>" 54)
+notation (ASCII output) bind_doN (infixr ">>=" 54)
+
+
+nonterminal doN_binds and doN_bind
+syntax
+  "_doN_block" :: "doN_binds \<Rightarrow> 'a" ("doN {//(2  _)//}" [12] 62)
+  "_doN_bind"  :: "[pttrn, 'a] \<Rightarrow> doN_bind" ("(2_ \<leftarrow>/ _)" 13)
+  "_doN_let" :: "[pttrn, 'a] \<Rightarrow> doN_bind" ("(2let _ =/ _)" [1000, 13] 13)
+  "_doN_then" :: "'a \<Rightarrow> doN_bind" ("_" [14] 13)
+  "_doN_final" :: "'a \<Rightarrow> doN_binds" ("_")
+  "_doN_cons" :: "[doN_bind, doN_binds] \<Rightarrow> doN_binds" ("_;//_" [13, 12] 12)
+  "_thenM" :: "['a, 'b] \<Rightarrow> 'c" (infixr "\<then>" 54)
+
+syntax (ASCII)
+  "_doN_bind" :: "[pttrn, 'a] \<Rightarrow> doN_bind" ("(2_ <-/ _)" 13)
+  "_thenM" :: "['a, 'b] \<Rightarrow> 'c" (infixr ">>" 54)
+
+translations
+  "_doN_block (_doN_cons (_doN_then t) (_doN_final e))"
+    \<rightleftharpoons> "CONST bind_doN t (\<lambda>_. e)"
+  "_doN_block (_doN_cons (_doN_bind p t) (_doN_final e))"
+    \<rightleftharpoons> "CONST bind_doN t (\<lambda>p. e)"
+  "_doN_block (_doN_cons (_doN_let p t) bs)"
+    \<rightleftharpoons> "let p = t in _doN_block bs"
+  "_doN_block (_doN_cons b (_doN_cons c cs))"
+    \<rightleftharpoons> "_doN_block (_doN_cons b (_doN_final (_doN_block (_doN_cons c cs))))"
+  "_doN_cons (_doN_let p t) (_doN_final s)"
+    \<rightleftharpoons> "_doN_final (let p = t in s)"
+  "_doN_block (_doN_final e)" \<rightharpoonup> "e"
+  "(m \<then> n)" \<rightharpoonup> "(m \<bind> (\<lambda>_. n))"
+  
+  
+definition [enres_unfolds]: "efor (lb::int) ub f \<sigma> \<equiv> doE {
+  EASSERT (lb\<le>ub);
+  (_,\<sigma>) \<leftarrow> EWHILET (\<lambda>(i,\<sigma>). i<ub) (\<lambda>(i,\<sigma>). doE { \<sigma> \<leftarrow> f i \<sigma>; ERETURN (i+1,\<sigma>) }) (lb,\<sigma>);
+  ERETURN \<sigma>
+}"  
+  
+thm EWHILEIT_rule
+
+  
+lemma efor_rule:
+  assumes INTV: "lb\<le>ub"
+  assumes I0: "I lb \<sigma>0"
+  assumes IS: "\<And>i \<sigma>. \<lbrakk> lb\<le>i; i<ub; I i \<sigma> \<rbrakk> \<Longrightarrow> f i \<sigma> \<le> ESPEC E (I (i+1))"
+  assumes FC: "\<And>\<sigma>. \<lbrakk> I ub \<sigma> \<rbrakk> \<Longrightarrow> P \<sigma>"
+  shows "efor lb ub f \<sigma>0 \<le> ESPEC E P"
+  unfolding efor_def
+  supply EWHILET_rule[where R="measure (\<lambda>(i,_). nat (ub-i))" and I="\<lambda>(i,\<sigma>). lb\<le>i \<and> i\<le>ub \<and> I i \<sigma>", refine_vcg]
+  apply refine_vcg
+  apply auto
+  using assms apply auto
+  done
+  
+
 
 end
